# 1

(a) $p \to \lnot q$

(b) $p \lor \lnot q$

(c) $p \to ((q \land \lnot r) \lor (\lnot q \land r))$

(d) $p \to ((q \land r) \lor (\lnot q \land \lnot r))$

(e) $p \to (q \land r)$

(f) $p \to q$

(g) $p \to (q \lor r)$

(h) $(p \land \lnot q) \lor (\lnot p \land q)$

(i) $p \to ((q \land \lnot r) \lor (\lnot q \land r))$

(j) $\lnot p \land \lnot q \land \lnot r$

(k) $p \land q$

# 2

(a) $((\lnot p) \land q) \to r$

(b) $(p \to q) \land (\lnot((r \lor p)\to q))$

(c) $(p \to q) \to (r \to (s \lor t))$

(d) $p \lor ((\lnot q) \to (p \land r))$

(e) $(p \land q) \to ((\lnot p) \land r)$

(f) $(p \lor p) \to (\lnot q)$

(g)